theories/poly/utp_poly_designs.thy
@@ -1,0 +1,185 @@
+(******************************************************************************)
+(* Project: Mechanisation of the UTP                                          *)
+(* File: utp_designs.thy                                                      *)
+(* Authors: Simon Foster, University of York                                  *)
+(******************************************************************************)
+
+header {* UTP Designs *}
+
+theory utp_poly_designs
+imports 
+  "../tactics/utp_rel_tac"
+  "../tactics/utp_xrel_tac"
+  "../tactics/utp_expr_tac"
+  "../core/utp_wp"
+  "../laws/utp_pred_laws"
+  "../laws/utp_rename_laws"
+  "../laws/utp_subst_laws"
+  "../laws/utp_rel_laws"
+  "../parser/utp_poly_parser"
+begin
+
+text {* Most predicates need a boolean type, so we here set the appropriate sort constraint *}
+
+default_sort BOOL_SORT
+
+abbreviation "okay  \<equiv> MkPVAR (bName ''okay'') True TYPE(bool) TYPE('m :: BOOL_SORT)"
+abbreviation "ok    \<equiv> PVarPE okay"
+abbreviation "ok'   \<equiv> PVarPE okay\<acute>"
+abbreviation "ok''  \<equiv> PVarPE okay\<acute>\<acute>"
+abbreviation "ok''' \<equiv> PVarPE okay\<acute>\<acute>\<acute>"
+abbreviation "OKAY \<equiv> {[okay]\<^sub>*,[okay\<acute>]\<^sub>*}"
+
+definition DesignD :: 
+"(bool, 'm) WF_PEXPRESSION \<Rightarrow>
+ (bool, 'm) WF_PEXPRESSION \<Rightarrow>
+ (bool, 'm) WF_PEXPRESSION" (infixr "\<turnstile>" 60) where
+"p \<turnstile> q = \<parallel>ok \<and> p \<Rightarrow> ok' \<and> q\<parallel>"
+
+syntax
+  "_upred_design" :: "pexpr \<Rightarrow> pexpr \<Rightarrow> pexpr" (infixr "\<turnstile>" 30)
+
+translations
+  "_upred_design p q"  == "CONST DesignD p q"
+
+term "\<parallel>true \<turnstile> II\<^bsub>REL_VAR - OKAY\<^esub>\<parallel>"
+
+definition SkipD :: "(bool, 'a) WF_PEXPRESSION" where
+"SkipD = \<parallel>true \<turnstile> II\<^bsub>REL_VAR - OKAY\<^esub>\<parallel>"
+
+notation SkipD ("II\<^sub>D")
+
+declare DesignD_def [eval,evalr,evalrx]
+declare SkipD_def [eval,evalr,evalrx]
+
+subsection {* Closure / UNREST theorems *}
+
+lemma MkPVAR_UNDASHED [simp]: 
+  "[MkPVAR (bName x) s a m]\<^sub>* \<in> UNDASHED"
+  by (simp add:PVAR_VAR_MkPVAR)
+
+lemma MkPVAR_aux [simp]:
+  "aux [MkPVAR n s a m]\<^sub>* = s"
+  by (simp add:PVAR_VAR_MkPVAR)
+
+lemma UNREST_PExprP [unrest]:
+  "UNREST_PEXPR vs e \<Longrightarrow> UNREST vs (PExprP e)"
+  by (auto simp add:UNREST_def UNREST_PEXPR_def PExprP_def)
+
+lemma UNREST_SkipD_NON_REL_VAR [unrest]:
+  "UNREST NON_REL_VAR II\<^sub>D"
+  apply (simp add:SkipD_def DesignD_def evalp)
+  apply (force intro: unrest)
+done
+
+
+lemma DesignD_rel_closure [closure]:
+  "\<lbrakk>``P`` \<in> WF_RELATION; ``Q`` \<in> WF_RELATION\<rbrakk> \<Longrightarrow> ``P \<turnstile> Q`` \<in> WF_RELATION"
+  by (simp add:DesignD_def closure evalp)
+
+lemma SkipD_rel_closure [closure]:
+  "``II\<^sub>D`` \<in> WF_RELATION"
+  apply (auto intro:closure simp add:SkipD_def evalp)
+  apply (rule closure)
+
+subsection {* Design Laws *}
+
+lemma DesignD_extreme_point_true:
+  "``false \<turnstile> false`` = ``false \<turnstile> true``"
+  by (utp_pred_tac)
+
+lemma DesignD_extreme_point_nok:
+  "``true \<turnstile> false`` = ``\<not> ok``"
+  by (utp_pred_tac)
+
+lemma DesignD_export_precondition:
+  "``P \<turnstile> Q`` = ``P \<turnstile> P \<and> Q``"
+  by (utp_pred_tac)
+
+text {* Design refinement law *}
+
+lemma EvalPE_UNREST_upd [simp]:
+  "\<lbrakk> UNREST_PEXPR vs e; v \<rhd> x; x \<in> vs \<rbrakk> \<Longrightarrow> \<lbrakk>e\<rbrakk>\<^sub>* (b(x :=\<^sub>b v)) = \<lbrakk>e\<rbrakk>\<^sub>* b"
+  apply (auto simp add:UNREST_PEXPR_def)
+  apply (metis binding_upd_override)
+done
+
+lemma SubstP_PExprP_UNREST [usubst]:
+  "\<lbrakk> UNREST_PEXPR vs e; v \<rhd>\<^sub>e x; x \<in> vs \<rbrakk> \<Longrightarrow> (PExprP e)[v|x] = PExprP e"
+  by (utp_pred_auto_tac)
+
+lemma DesignD_refinement:
+  assumes "UNREST_PEXPR OKAY P1" "UNREST_PEXPR OKAY P2"
+          "UNREST_PEXPR OKAY Q1" "UNREST_PEXPR OKAY Q2"
+  shows "``P1 \<turnstile> Q1 \<sqsubseteq> P2 \<turnstile> Q2`` = ``[P1 \<Rightarrow> P2] \<and> [P1 \<and> Q2 \<Rightarrow> Q1]``"
+proof -
+  have "``(P1 \<turnstile> Q1) \<sqsubseteq> (P2 \<turnstile> Q2)`` = ``[P2 \<turnstile> Q2 \<Rightarrow> P1 \<turnstile> Q1]``"
+    by (utp_pred_tac)
+
+  also have "... = ``[(ok \<and> P2 \<Rightarrow> ok' \<and> Q2) \<Rightarrow> (ok \<and> P1 \<Rightarrow> ok' \<and> Q1)]``"
+    by (utp_pred_tac)
+
+  also with assms have "... = ``[(P2 \<Rightarrow> ok' \<and> Q2) \<Rightarrow> (P1 \<Rightarrow> ok' \<and> Q1)]``"
+    apply (simp add:evalp)
+    apply (rule_tac trans)
+    apply (rule_tac x="[okay]\<^sub>*" in BoolType_aux_var_split_taut)
+    apply (simp_all add:usubst typing defined unrest)
+  done
+
+  also from assms have "... = `[(\<not> P2 \<Rightarrow> \<not> P1) \<and> ((P2 \<Rightarrow> Q2) \<Rightarrow> (P1 \<Rightarrow> Q1))]`"
+    apply (simp add:evalp)
+    apply (rule_tac trans)
+    apply (rule_tac x="[okay\<acute>]\<^sub>*" in BoolType_aux_var_split_taut)
+    apply (simp_all add:usubst typing defined)
+  done
+
+  also have "... = `[(P1 \<Rightarrow> P2) \<and> ((P2 \<Rightarrow> Q2) \<Rightarrow> (P1 \<Rightarrow> Q1))]`"
+    by (utp_pred_auto_tac)
+
+  also have "... = `[(P1 \<Rightarrow> P2)] \<and> [P1 \<and> Q2 \<Rightarrow> Q1]`"
+    by (utp_pred_auto_tac)
+
+  ultimately show ?thesis
+    by (metis (hide_lams, no_types) PredPE_inv)
+qed
+
+lemma SubstPE_AndPE [usubst]:
+  "``(P \<and> Q)[v/x]`` = ``P[v/x] \<and> Q[v/x]``"
+  by (utp_pred_tac)
+
+lemma SubstPE_ImpliesPE [usubst]:
+  "``(P \<Rightarrow> Q)[v/x]`` = ``P[v/x] \<Rightarrow> Q[v/x]``"
+  by (utp_pred_tac)
+
+lemma [simp]: 
+  "``false \<Rightarrow> p`` = ``true``"
+  "``false \<and> p`` = ``false``"
+  by (utp_pred_tac+)
+
+lemma DesignD_diverge:
+  "``(P \<turnstile> Q)[false/okay]`` = ``true``"
+  by (simp add:DesignD_def usubst typing defined)
+
+lemma DesignD_left_zero:
+  assumes "P \<in> WF_RELATION" "Q \<in> WF_RELATION"
+  shows "true ; (P \<turnstile> Q) = true"
+proof -
+
+  from assms have "`true ; (P \<turnstile> Q)` = `\<exists> okay\<acute>\<acute>\<acute>. true[$okay\<acute>\<acute>\<acute>/okay\<acute>] ; (P \<turnstile> Q)[$okay\<acute>\<acute>\<acute>/okay]`"
+    by (simp add: SemiR_extract_variable closure)
+
+  also from assms have "... = `(true[false/okay\<acute>] ; (P \<turnstile> Q)[false/okay]) \<or> (true[true/okay\<acute>] ; (P \<turnstile> Q)[true/okay])`"
+    apply (rule_tac trans)
+    apply (rule BoolType_aux_var_split_exists, simp_all)
+    apply (simp add:usubst typing assms closure defined unrest)
+  done
+
+  also have "... = `((true ; true) \<or> (true ; ((P \<turnstile> Q)[true/okay])))`"
+    by (simp add:usubst closure typing DesignD_diverge)
+
+  ultimately show ?thesis
+    by (simp add:closure SemiR_TrueP_precond)
+qed
+
+
+end
